pipit/plugin-test/Pipit.Plugin.Check.fst
@@ -1,3 +1,4 @@
+// TODO move this to plugin/
 module Pipit.Plugin.Check
 
 module PPL = Pipit.Plugin.Lift
