Makefile
@@ -18,12 +18,10 @@ include make/pipit/abstract.mk
 include make/pipit/extract.mk
 include make/pipit/source.mk
 
-#XXXNOCOMMIT
-# include make/pipit/example.mk
-# include make/pipit/test.mk
+include make/pipit/example.mk
+include make/pipit/test.mk
 
 include make/pipit/plugin.mk
-#XXXNOCOMMIT
 # FSTAR_EXTRA_OPT:=$(FSTAR_EXTRA_OPT) --debug Plugin.Test.Language.Lift --ext pipit:lift:debug=1
 include make/pipit/plugin-test.mk
 
